src/QL/FOL/language.lean
@@ -5,7 +5,7 @@ universes u v
 namespace fol
 open_locale logic_symbol aclogic
 open subterm subformula logic logic.Theory
-variables {L R : language.{u}} {L₁ L₂ L₃ : language} {m n : ℕ}
+variables {L R : language.{u}} {L₁ L₂ L₃ : language} {n : ℕ}
 
 namespace language
 
@@ -74,7 +74,7 @@ end padd
 section Constants
 variables {α : Type*}
 
-instance : has_coe α (subterm (Constants α) m n) := ⟨subterm.const (Constants α)⟩
+instance : has_coe α (subterm (Constants α) n) := ⟨subterm.const (Constants α)⟩
 
 end Constants
 
@@ -84,58 +84,58 @@ namespace subterm
 open language
 
 structure hom (L₁ : language) (L₂ : language) :=
-(func {} : Π {k m n}, L₁.fn k → (fin k → subterm L₂ m n) → subterm L₂ m n)
-(to_fun : Π {m n}, subterm L₁ m n → subterm L₂ m n)
-(map_var' : ∀ {m n x}, to_fun (#x : subterm L₁ m n) = #x)
-(map_metavar' : ∀ {m n x}, to_fun (&x : subterm L₁ m n) = &x)
-(map_function' : ∀ {k m n} (f : L₁.fn k) (v : fin k → subterm L₁ m n),
+(func {} : Π {k n}, L₁.fn k → (fin k → subterm L₂ n) → subterm L₂ n)
+(to_fun : Π {n}, subterm L₁ n → subterm L₂ n)
+(map_var' : ∀ {n x}, to_fun (#x : subterm L₁ n) = #x)
+(map_metavar' : ∀ {n x}, to_fun (&x : subterm L₁ n) = &x)
+(map_function' : ∀ {k n} (f : L₁.fn k) (v : fin k → subterm L₁ n),
   to_fun (function f v) = func f (to_fun ∘ v))
-(map_mlift' : ∀ {m n} (t : subterm L₁ m n), to_fun t.mlift = (to_fun t).mlift)
-(map_push' : ∀ {m n} (t : subterm L₁ m (n + 1)), to_fun t.push = (to_fun t).push)
-(map_pull' : ∀ {m n} (t : subterm L₁ (m + 1) n), to_fun t.pull = (to_fun t).pull)
+(map_mlift' : ∀ {n} (t : subterm L₁ n), to_fun t.mlift = (to_fun t).mlift)
+(map_push' : ∀ {n} (t : subterm L₁ (n + 1)), to_fun t.push = (to_fun t).push)
+(map_pull' : ∀ {n} (t : subterm L₁ n), to_fun t.pull = (to_fun t).pull)
 
 instance {L₁ L₂ : language} :
-  has_coe_to_fun (hom L₁ L₂) (λ _, Π {m n}, subterm L₁ m n → subterm L₂ m n) :=
+  has_coe_to_fun (hom L₁ L₂) (λ _, Π {n}, subterm L₁ n → subterm L₂ n) :=
 ⟨hom.to_fun⟩
 
 namespace hom
-variables {L₁ L₂} {m n} (τ : hom L₁ L₂)
+variables {L₁ L₂ n} (τ : hom L₁ L₂)
 
-@[simp] lemma map_var {m n x} : τ (#x : subterm L₁ m n) = #x := τ.map_var'
+@[simp] lemma map_var {n x} : τ (#x : subterm L₁ n) = #x := τ.map_var'
 
-@[simp] lemma map_metavar {m n x} : τ (&x : subterm L₁ m n) = &x := τ.map_metavar'
+@[simp] lemma map_metavar {n x} : τ (&x : subterm L₁ n) = &x := τ.map_metavar'
 
-lemma map_function {k m n} (f : L₁.fn k) (v : fin k → subterm L₁ m n) :
+lemma map_function {k n} (f : L₁.fn k) (v : fin k → subterm L₁ n) :
   τ (function f v) = func τ f (λ i, τ (v i)) := τ.map_function' f v
 
-@[simp] lemma map_mlift {m n} (t : subterm L₁ m n) : τ t.mlift = (τ t).mlift := τ.map_mlift' t
+@[simp] lemma map_mlift {n} (t : subterm L₁ n) : τ t.mlift = (τ t).mlift := τ.map_mlift' t
 
-@[simp] lemma map_push {m n} (t : subterm L₁ m (n + 1)) : τ t.push = (τ t).push := τ.map_push' t
+@[simp] lemma map_push {n} (t : subterm L₁ (n + 1)) : τ t.push = (τ t).push := τ.map_push' t
 
-@[simp] lemma map_pull {m n} (t : subterm L₁ (m + 1) n) : τ t.pull = (τ t).pull := τ.map_pull' t
+@[simp] lemma map_pull {n} (t : subterm L₁ n) : τ t.pull = (τ t).pull := τ.map_pull' t
 
 end hom
 
-@[simp] def of_fn_hom (fn : Π n, L₁.fn n → L₂.fn n) : subterm L₁ m n → subterm L₂ m n
+@[simp] def of_fn_hom (fn : Π n, L₁.fn n → L₂.fn n) : subterm L₁ n → subterm L₂ n
 | &x             := &x
 | #x             := #x
 | (function f v) := function (fn _ f) (λ i, of_fn_hom (v i))
 
 def of_fn (fn : Π n, L₁.fn n → L₂.fn n) : hom L₁ L₂ :=
-{ func := λ k m n f, function (fn _ f),
-  to_fun := λ m n, @of_fn_hom _ _ m n fn,
+{ func := λ k n f, function (fn k f),
+  to_fun := λ n, @of_fn_hom _ _ n fn,
   map_var' := by intros; refl,
   map_metavar' := by intros; refl,
   map_function' := by intros; simp,
-  map_mlift' := by intros m n t; induction t; simp*,
-  map_push' := by {intros m n t; induction t; simp*, case var : x { refine fin.last_cases _ _ x; simp } },
-  map_pull' := by {intros m n t; induction t; simp*, case metavar : x { refine fin.cases _ _ x; simp } } }
+  map_mlift' := by intros n t; induction t; simp*,
+  map_push' := by {intros n t; induction t; simp*, case var : x { refine fin.last_cases _ _ x; simp } },
+  map_pull' := by {intros n t; induction t; simp*, case metavar : x { cases x; simp } } }
 
 def of_lhom (l : L₁ ⤳ᴸ L₂) : hom L₁ L₂ := of_fn l.fn
 
 variables (l : L₁ ⤳ᴸ L₂)
 
-@[simp] lemma of_lhom_map_function {k m n} (f : L₁.fn k) (v : fin k → subterm L₁ m n) :
+@[simp] lemma of_lhom_map_function {k n} (f : L₁.fn k) (v : fin k → subterm L₁ n) :
   (of_lhom l) (function f v) = function (l.fn _ f) (λ i, of_lhom l (v i)) :=
 by simp[of_lhom]; refl
 
@@ -151,79 +151,79 @@ namespace subformula
 open language
 
 structure hom (L₁ : language) (L₂ : language) :=
-(hom : Π {m n}, subformula L₁ m n →ₗ subformula L₂ m n)
-(map_univ' : ∀ {m n} (p : subformula L₁ m (n + 1)), hom (∀'p) = ∀' hom p)
-(map_mlift' : ∀ {m n} (p : subformula L₁ m n), hom p.mlift = (hom p).mlift)
-(map_push' : ∀ {m n} (p : subformula L₁ m (n + 1)), hom p.push = (hom p).push)
-(map_pull' : ∀ {m n} (p : subformula L₁ (m + 1) n), hom p.pull = (hom p).pull)
+(hom : Π {n}, subformula L₁ n →ₗ subformula L₂ n)
+(map_univ' : ∀ {n} (p : subformula L₁ (n + 1)), hom (∀'p) = ∀' hom p)
+(map_mlift' : ∀ {n} (p : subformula L₁ n), hom p.mlift = (hom p).mlift)
+(map_push' : ∀ {n} (p : subformula L₁ (n + 1)), hom p.push = (hom p).push)
+(map_pull' : ∀ {n} (p : subformula L₁ n), hom p.pull = (hom p).pull)
 
 instance {L₁ L₂ : language} :
-  has_coe_to_fun (hom L₁ L₂) (λ _, Π {m n}, subformula L₁ m n →ₗ subformula L₂ m n) :=
+  has_coe_to_fun (hom L₁ L₂) (λ _, Π {n}, subformula L₁ n →ₗ subformula L₂ n) :=
 ⟨hom.hom⟩
 
 namespace hom
-variables (τ : subformula.hom L₁ L₂) {m}
+variables (τ : subformula.hom L₁ L₂) {n}
 
-@[simp] lemma map_univ {m n} (p : subformula L₁ m (n + 1)) : τ (∀'p) = ∀'τ p := τ.map_univ' p
+@[simp] lemma map_univ (p : subformula L₁ (n + 1)) : τ (∀'p) = ∀'τ p := τ.map_univ' p
 
-@[simp] lemma map_ex {m n} (p : subformula L₁ m (n + 1)) : τ (∃'p) = ∃'τ p := by simp[ex_def]
+@[simp] lemma map_ex (p : subformula L₁ (n + 1)) : τ (∃'p) = ∃'τ p := by simp[ex_def]
 
-@[simp] lemma map_mlift {m n} (p : subformula L₁ m n) : τ p.mlift = (τ p).mlift := τ.map_mlift' p
+@[simp] lemma map_mlift (p : subformula L₁ n) : τ p.mlift = (τ p).mlift := τ.map_mlift' p
 
-@[simp] lemma map_push {m n} (p : subformula L₁ m (n + 1)) : τ p.push = (τ p).push := τ.map_push' p
+@[simp] lemma map_push (p : subformula L₁ (n + 1)) : τ p.push = (τ p).push := τ.map_push' p
 
-@[simp] lemma map_pull {m n} (p : subformula L₁ (m + 1) n) : τ p.pull = (τ p).pull := τ.map_pull' p
+@[simp] lemma map_pull (p : subformula L₁ n) : τ p.pull = (τ p).pull := τ.map_pull' p
 
-@[simp] lemma map_dummy {m n} (p : subformula L₁ m n) : τ p.dummy = (τ p).dummy :=
+@[simp] lemma map_dummy (p : subformula L₁ n) : τ p.dummy = (τ p).dummy :=
 by simp[dummy]
 
-@[simp] lemma map_univ_closure {m n} (p : subformula L₁ m n) : τ (∀'*p) = ∀'*(τ p) :=
+@[simp] lemma map_univ_closure (p : subformula L₁ n) : τ (∀'*p) = ∀'*(τ p) :=
 by induction n; simp*
 
-@[simp] lemma map_exists_closure {m n} (p : subformula L₁ m n) : τ (∃'*p) = ∃'*(τ p) :=
+@[simp] lemma map_exists_closure (p : subformula L₁ n) : τ (∃'*p) = ∃'*(τ p) :=
 by induction n; simp*
 
-@[reducible] def on_Theory (T : preTheory L₁ m) : preTheory L₂ m := (λ p, τ p) '' T
+@[reducible] def on_Theory (T : preTheory L₁) : preTheory L₂ := (λ p, τ p) '' T
 
-@[simp] lemma on_Theory_map_mlift {m} (T : preTheory L₁ m) : τ.on_Theory T.mlift = (τ.on_Theory T).mlift :=
+@[simp] lemma on_Theory_map_mlift (T : preTheory L₁) : τ.on_Theory T.mlift = (τ.on_Theory T).mlift :=
 by ext p; simp[on_Theory, preTheory.mlift]
 
 class provable :=
-(subst : ∀ {m} (T : preTheory L₁ m) (p t), τ.on_Theory T ⊢ ∀'τ p ⟶ τ (subst t p))
+(subst : ∀ (T : preTheory L₁) (p t), τ.on_Theory T ⊢ ∀'τ p ⟶ τ (subst t p))
 
 end hom
 
-variables (l : L₁ ⤳ᴸ L₂) {m}
+variables (l : L₁ ⤳ᴸ L₂)
 
-@[simp] def of_lhom_hom : Π {n}, subformula L₁ m n → subformula L₂ m n
+@[simp] def of_lhom_hom : Π {n}, subformula L₁ n → subformula L₂ n
 | n verum          := ⊤
 | n (relation r v) := relation (l.pr _ r) (λ i, subterm.of_lhom l (v i))
 | n (imply p q)    := of_lhom_hom p ⟶ of_lhom_hom q
 | n (neg p)        := ∼of_lhom_hom p
 | n (fal p)        := ∀' of_lhom_hom p
 
-@[simp] def of_lhom_hom_verum : of_lhom_hom l (⊤ : subformula L₁ m n) = ⊤ := by refl
+@[simp] def of_lhom_hom_verum : of_lhom_hom l (⊤ : subformula L₁ n) = ⊤ := by refl
 
-@[simp] def of_lhom_hom_relation {k} (r : L₁.pr k) (v : fin k → subterm L₁ m n) :
-  of_lhom_hom l (relation r v : subformula L₁ m n) = relation (l.pr _ r) (λ i, subterm.of_lhom l (v i)) := by refl
+@[simp] def of_lhom_hom_relation {k} (r : L₁.pr k) (v : fin k → subterm L₁ n) :
+  of_lhom_hom l (relation r v : subformula L₁ n) = relation (l.pr _ r) (λ i, subterm.of_lhom l (v i)) := by refl
 
-@[simp] def of_lhom_hom_imply (p q : subformula L₁ m n) :
+@[simp] def of_lhom_hom_imply (p q : subformula L₁ n) :
   of_lhom_hom l (p ⟶ q) = (of_lhom_hom l p ⟶ of_lhom_hom l q) := by refl
 
-@[simp] def of_lhom_hom_neg (p : subformula L₁ m n) :
+@[simp] def of_lhom_hom_neg (p : subformula L₁ n) :
   of_lhom_hom l (∼p) = ∼of_lhom_hom l p := by refl
 
-@[simp] def of_lhom_hom_fal (p : subformula L₁ m (n + 1)) :
+@[simp] def of_lhom_hom_fal (p : subformula L₁ (n + 1)) :
   of_lhom_hom l (∀'p) = ∀'of_lhom_hom l p := by refl
 
-@[simp] def mlift_of_lhom_hom : Π {n} (p : subformula L₁ m n), mlift (of_lhom_hom l p) = of_lhom_hom l (mlift p)
+@[simp] def mlift_of_lhom_hom : Π {n} (p : subformula L₁ n), mlift (of_lhom_hom l p) = of_lhom_hom l (mlift p)
 | n verum          := by simp[top_eq]; refl
 | n (relation r v) := by simp
 | n (imply p q)    := by simp[imply_eq, mlift_of_lhom_hom p, mlift_of_lhom_hom q]
 | n (neg p)        := by simp[neg_eq, mlift_of_lhom_hom p]
 | n (fal p)        := by simp[fal_eq, mlift_of_lhom_hom p]
 
-@[simp] def push_of_lhom_hom : Π {n} (p : subformula L₁ m (n + 1)), push (of_lhom_hom l p) = of_lhom_hom l (push p)
+@[simp] def push_of_lhom_hom : Π {n} (p : subformula L₁ (n + 1)), push (of_lhom_hom l p) = of_lhom_hom l (push p)
 | n verum          := by simp[top_eq]; refl
 | n (relation r v) := by simp
 | n (imply p q)    := by simp[imply_eq, push_of_lhom_hom p, push_of_lhom_hom q]
@@ -231,7 +231,7 @@ variables (l : L₁ ⤳ᴸ L₂) {m}
 | n (fal p)        := by simp[fal_eq, push_of_lhom_hom p]
 using_well_founded {rel_tac := λ _ _, `[exact ⟨_, measure_wf (λ x, x.2.complexity)⟩]}
 
-@[simp] def pull_of_lhom_hom : Π {n} (p : subformula L₁ (m + 1) n), pull (of_lhom_hom l p) = of_lhom_hom l (pull p)
+@[simp] def pull_of_lhom_hom : Π {n} (p : subformula L₁ n), pull (of_lhom_hom l p) = of_lhom_hom l (pull p)
 | n verum          := by simp[top_eq]; refl
 | n (relation r v) := by simp
 | n (imply p q)    := by simp[imply_eq, pull_of_lhom_hom p, pull_of_lhom_hom q]
@@ -239,7 +239,7 @@ using_well_founded {rel_tac := λ _ _, `[exact ⟨_, measure_wf (λ x, x.2.compl
 | n (fal p)        := by simp[fal_eq, pull_of_lhom_hom p]
 
 def of_lhom : subformula.hom L₁ L₂ :=
-{ hom := λ m n,
+{ hom := λ n,
   { to_fun := of_lhom_hom l,
     map_neg' := λ p, by refl,
     map_imply' := λ p q, by refl,
@@ -247,26 +247,26 @@ def of_lhom : subformula.hom L₁ L₂ :=
     map_or' := λ p q, by refl,
     map_top' := by refl,
     map_bot' := by refl },
-  map_univ' := λ m n p, by refl,
+  map_univ' := λ n p, by refl,
   map_mlift' := by simp,
   map_push' := by simp,
   map_pull' := by simp }
 
-@[simp] lemma of_lhom_relation {k} (r : L₁.pr k) (v : fin k → subterm L₁ m n) :
+@[simp] lemma of_lhom_relation {k} (r : L₁.pr k) (v : fin k → subterm L₁ n) :
   of_lhom l (relation r v) = relation (l.pr _ r) (λ i, (subterm.of_lhom l) (v i)) :=
 by refl
 
-@[simp] lemma rank_of_lhom : ∀ {n} (p : subformula L₁ m n), (of_lhom l p).qr = p.qr
+@[simp] lemma rank_of_lhom : ∀ {n} (p : subformula L₁ n), (of_lhom l p).qr = p.qr
 | n verum          := by simp[top_eq]
 | n (relation r v) := by simp
 | n (imply p q)    := by simp[imply_eq, rank_of_lhom p, rank_of_lhom q]
 | n (neg p)        := by simp[neg_eq, rank_of_lhom p]
 | n (fal p)        := by simp[fal_eq, rank_of_lhom p]
 
-@[simp] lemma of_lhom_is_open (p : subformula L₁ m n) : (of_lhom l p).is_open ↔ p.is_open :=
+@[simp] lemma of_lhom_is_open (p : subformula L₁ n) : (of_lhom l p).is_open ↔ p.is_open :=
 by simp[is_open]
 
-@[simp] lemma complexity_of_lhom : ∀ {n} (p : subformula L₁ m n), (of_lhom l p).complexity = p.complexity
+@[simp] lemma complexity_of_lhom : ∀ {n} (p : subformula L₁ n), (of_lhom l p).complexity = p.complexity
 | n verum          := by simp[top_eq]
 | n (relation r v) := by simp
 | n (imply p q)    := by simp[imply_eq, complexity_of_lhom p, complexity_of_lhom q]
