src/QL/FOL/semantics.lean
@@ -18,53 +18,53 @@ variables {L : language.{u}} {S : Structure L}
 
 instance (S : Structure L) : inhabited S.dom := S.dom_inhabited
 
-variables (S) {m n : ℕ}
+variables (S) {n : ℕ}
 
 open subterm subformula
 
 namespace  subterm
-variables {m} {m₁ m₂ : ℕ} {n} (me : fin m → S) (e : fin n → S)
+variables {n} (me : ℕ → S) (e : fin n → S)
 
-@[simp] def val (me : fin m → S) (e : fin n → S) : subterm L m n → S
+@[simp] def val (me : ℕ → S) (e : fin n → S) : subterm L n → S
 | (&x)           := me x
 | (#x)           := e x
 | (function f v) := S.fn f (λ i, (v i).val)
 
-lemma val_rew (s : finitary (subterm L m₂ n) m₁) (me : fin m₂ → S) (e : fin n → S) : ∀ (t : subterm L m₁ n),
+lemma val_rew (s : ℕ → subterm L n) (me : ℕ → S) (e : fin n → S) : ∀ (t : subterm L n),
   (rew s t).val S me e = t.val S (val S me e ∘ s) e
 | (&x)           := by simp
 | (#x)           := by simp
 | (function f v) := by simp; refine congr_arg _ (by ext i; exact val_rew (v i))
 
-@[simp] lemma val_mlift (x : S) (t : subterm L m n) :
-  t.mlift.val S (x *> me) e = t.val S me e :=
+@[simp] lemma val_mlift (x : S) (t : subterm L n) :
+  t.mlift.val S (x .> me) e = t.val S me e :=
 by simp[mlift_eq_rew, val_rew]; congr; ext x; simp
 
-@[simp] lemma val_lift (x : S) (t : subterm L m n) :
+@[simp] lemma val_lift (x : S) (t : subterm L n) :
   t.lift.val S me (x *> e) = t.val S me e :=
 by induction t; simp*
 
-@[simp] lemma val_push (me : fin m → S) (x : S) (e : fin n → S) (t : subterm L m (n + 1)) :
-  val S (x *> me) e t.push = val S me (e <* x) t :=
+@[simp] lemma val_push (x : S) (e : fin n → S) (t : subterm L (n + 1)) :
+  val S (x .> me) e t.push = val S me (e <* x) t :=
 by { induction t; simp*, case var : u { refine fin.last_cases _ _ u; simp } }
 
-@[simp] lemma val_pull (me : fin m → S) (x : S) (e : fin n → S) (t : subterm L (m + 1) n) :
-  val S me (e <* x) t.pull = val S (x *> me) e t :=
-by { induction t; simp*, case metavar : u { refine fin.cases _ _ u; simp } }
+@[simp] lemma val_pull (x : S) (e : fin n → S) (t : subterm L n) :
+  val S me (e <* x) t.pull = val S (x .> me) e t :=
+by { induction t; simp*, case metavar : u { cases u; simp } }
 
 end  subterm
 
 namespace subformula
-variables {m₁ m₂ : ℕ} {n} (me : fin m → S) (e : fin n → S)
+variables {n} (me : ℕ → S) (e : fin n → S)
 
-@[simp] def val' (me : fin m → S) : ∀ {n} (e : fin n → S), subformula L m n → Prop
+@[simp] def val' (me : ℕ → S) : ∀ {n} (e : fin n → S), subformula L n → Prop
 | n _ verum          := true
 | n e (relation p v) := S.pr p (subterm.val S me e ∘ v)
 | n e (imply p q)    := p.val' e → q.val' e
 | n e (neg p)        := ¬(p.val' e)
 | n e (fal p)        := ∀ x : S.dom, (p.val' (x *> e))
 
-@[irreducible] def val (me : fin m → S) (e : fin n → S) : subformula L m n →ₗ Prop :=
+@[irreducible] def val (me : ℕ → S) (e : fin n → S) : subformula L n →ₗ Prop :=
 { to_fun := val' S me e,
   map_neg' := λ _, by refl,
   map_imply' := λ _ _, by refl,
@@ -76,10 +76,10 @@ variables {m₁ m₂ : ℕ} {n} (me : fin m → S) (e : fin n → S)
 @[simp] lemma val_relation {p} (r : L.pr p) (v) :
   val S me e (relation r v) ↔ S.pr r (subterm.val S me e ∘ v) :=  by simp[val]; refl
 
-@[simp] lemma val_fal (p : subformula L m (n + 1)) :
+@[simp] lemma val_fal (p : subformula L (n + 1)) :
   val S me e (∀'p) ↔ ∀ x : S, val S me (x *> e) p := by simp[val]; refl
 
-lemma val_rew (me : fin m₂ → S) : ∀ {n} (e : fin n → S) (s : finitary (subterm L m₂ n) m₁) (p : subformula L m₁ n),
+lemma val_rew : ∀ {n} (e : fin n → S) (s : ℕ → subterm L n) (p : subformula L n),
   val S me e (rew s p) ↔ val S (subterm.val S me e ∘ s) e p
 | n e s (relation r v) := by simp[subterm.val_rew]; refine iff_of_eq (congr_arg _ (by ext x; simp[subterm.val_rew]))
 | n e s verum          := by simp[top_eq]
@@ -90,14 +90,14 @@ lemma val_rew (me : fin m₂ → S) : ∀ {n} (e : fin n → S) (s : finitary (s
         have : (subterm.val S me (x *> e) ∘ subterm.lift ∘ s) = subterm.val S me e ∘ s, by funext x; simp,
         rw this }
  
-@[simp] lemma val_mlift (e : fin n → S) (x : S) (p : subformula L m n) :
-  val S (x *> me) e p.mlift = val S me e p :=
+@[simp] lemma val_mlift (e : fin n → S) (x : S) (p : subformula L n) :
+  val S (x .> me) e p.mlift = val S me e p :=
 by { simp[mlift_eq_rew, val_rew],
-     have : subterm.val S (x *> me) e ∘ metavar ∘ fin.succ = me, by funext x; simp,
+     have : subterm.val S (x .> me) e ∘ metavar ∘ nat.succ = me, by funext x; simp,
      rw this }
 
-@[simp] lemma val_push (x : S) : ∀ {n} (e : fin n → S) (p : subformula L m (n + 1)),
-  val S (x *> me) e p.push ↔ val S me (e <* x) p
+@[simp] lemma val_push (x : S) : ∀ {n} (e : fin n → S) (p : subformula L (n + 1)),
+  val S (x .> me) e p.push ↔ val S me (e <* x) p
 | n e (relation r v) := by simp; refine iff_of_eq (congr_arg _ $ funext $ by simp)
 | n e verum          := by simp[top_eq]
 | n e (imply p q)    := by simp[imply_eq, val_push _ p, val_push _ q]
@@ -106,8 +106,8 @@ by { simp[mlift_eq_rew, val_rew],
   { intros y, simp[fin.left_right_concat_assoc], exact val_push (y *> e) p} }
 using_well_founded {rel_tac := λ _ _, `[exact ⟨_, measure_wf (λ x, x.2.2.complexity)⟩]}
 
-@[simp] lemma val_pull (x : S) : ∀ {n} (e : fin n → S) (p : subformula L (m + 1) n),
-  val S me (e <* x) p.pull ↔ val S (x *> me) e p
+@[simp] lemma val_pull (x : S) : ∀ {n} (e : fin n → S) (p : subformula L n),
+  val S me (e <* x) p.pull ↔ val S (x .> me) e p
 | n e (relation r v) := by simp; refine iff_of_eq (congr_arg _ $ funext $ by simp)
 | n e verum          := by simp[top_eq]
 | n e (imply p q)    := by simp[imply_eq, val_pull _ p, val_pull _ q]
@@ -115,25 +115,25 @@ using_well_founded {rel_tac := λ _ _, `[exact ⟨_, measure_wf (λ x, x.2.2.com
 | n e (fal p)        := by { simp[fal_eq], refine forall_congr _,
   { intros y, simp[fin.left_right_concat_assoc], exact val_pull (y *> e) p} }
 
-@[simp] lemma val_dummy (x : S) : ∀ {n} (e : fin n → S) (p : subformula L m n),
+@[simp] lemma val_dummy (x : S) : ∀ {n} (e : fin n → S) (p : subformula L n),
   val S me (e <* x) p.dummy ↔ val S me e p :=
 by simp[dummy]
 
-@[simp] lemma val_msubst (p : subformula L (m + 1) n) (t : subterm L m n) :
-  val S me e (msubst t p) ↔ val S (subterm.val S me e t *> me) e p :=
-by simp[msubst, val_rew, fin.comp_left_concat, show subterm.val S me e ∘ metavar = me, from funext (by simp)]
+@[simp] lemma val_msubst (p : subformula L n) (t : subterm L n) :
+  val S me e (msubst t p) ↔ val S (subterm.val S me e t .> me) e p :=
+by simp[msubst, val_rew, nat.comp_left_concat, show subterm.val S me e ∘ metavar = me, from funext (by simp)]
 
-@[simp] lemma val_subst (p : subformula L m (n + 1)) (t : subterm L m n) :
+@[simp] lemma val_subst (p : subformula L (n + 1)) (t : subterm L n) :
   val S me e (subst t p) ↔ val S me (e <* subterm.val S me e t) p :=
 by simp[subst, val_msubst]
 
-@[simp] lemma val_substs (p : subformula L m n) (v : fin n → subterm L m 0) :
+@[simp] lemma val_substs (p : subformula L n) (v : fin n → subterm L 0) :
   val S me fin.nil (substs v p) ↔ val S me (subterm.val S me fin.nil ∘ v) p :=
-by { induction n with n IH generalizing m; simp[substs],
+by { induction n with n IH generalizing me; simp[substs],
   { rw[show subterm.val S me fin.nil ∘ v = fin.nil, by simp] },
   { simp[IH, (∘), ←fin.comp_right_concat] } }
 
-@[simp] lemma val_universal_closure (p : subformula L m n) :
+@[simp] lemma val_universal_closure (p : subformula L n) :
   val S me fin.nil (∀'* p) ↔ ∀ v, val S me v p :=
 begin
   induction n with n IH,
@@ -143,10 +143,10 @@ begin
     { intros h v x, exact h (x *> v) } }
 end
 
-@[simp] lemma val_ex (p : subformula L m (n + 1)) :
+@[simp] lemma val_ex (p : subformula L (n + 1)) :
   val S me e (∃'p) ↔ ∃ x : S, val S me (x *> e) p := by simp[ex_def]
 
-@[simp] lemma val_exists_closure (p : subformula L m n) :
+@[simp] lemma val_exists_closure (p : subformula L n) :
   val S me fin.nil (∃'*p) ↔ ∃ v, val S me v p :=
 begin
   induction n with n IH,
@@ -159,101 +159,74 @@ end
 
 end subformula
 
-class Structure.proper_equal [L.has_equal] {me e} (t u : subterm L m n)
+class Structure.proper_equal [L.has_equal] {me e} (t u : subterm L n)
 (val_eq : subformula.val S me e (t =' u) ↔ (t.val S me e = u.val S me e))
 
 namespace formula
-variables (S) {me : fin m → S}
+variables (S) {me : ℕ → S}
 
-@[reducible] def val (me : fin m → S) : formula L m →ₗ Prop := subformula.val S me fin.nil
+@[reducible] def val (me : ℕ → S) : formula L →ₗ Prop := subformula.val S me fin.nil
 
 notation S` ⊧[`:80 e`] `p :50 := val S e p
 
-variables {S} {p q : formula L m}
+variables {S} {p q : formula L}
 
 @[simp] lemma models_relation {k} {r : L.pr k} {v} :
   S ⊧[me] relation r v ↔ S.pr r (subterm.val S me fin.nil ∘ v) := by simp[val]
 
-@[simp] lemma models_fal {p : subformula L m 1} :
-  S ⊧[me] (∀'p : subformula _ _ _) ↔ ∀ x, S ⊧[x *> me] p.push :=
+@[simp] lemma models_fal {p : subformula L 1} :
+  S ⊧[me] ∀'p ↔ ∀ x, S ⊧[x .> me] p.push :=
 by simp[val, fin.concat_zero]
 
-@[simp] lemma models_ex {p : subformula L m 1} :
-  S ⊧[me] (∃'p : subformula _ _ _) ↔ ∃ x, S ⊧[x *> me] p.push :=
+@[simp] lemma models_ex {p : subformula L 1} :
+  S ⊧[me] ∃'p ↔ ∃ x, S ⊧[x .> me] p.push :=
 by simp[val, fin.concat_zero]
 
-@[simp] lemma models_subst {p : subformula L m 1} (t : subterm L m 0) :
-  S ⊧[me] (subst t p : subformula _ _ _) ↔ S ⊧[subterm.val S me fin.nil t *> me] p.push :=
+@[simp] lemma models_subst {p : subformula L 1} (t : subterm L 0) :
+  S ⊧[me] (subst t p) ↔ S ⊧[subterm.val S me fin.nil t .> me] p.push :=
 by simp[val, subformula.val_subst]
 
-@[simp] lemma modfels_substs (p : subformula L m n) (v : fin n → subterm L m 0) :
+@[simp] lemma modfels_substs (p : subformula L n) (v : fin n → subterm L 0) :
   S ⊧[me] substs v p ↔ subformula.val S me (subterm.val S me fin.nil ∘ v) p :=
 by simp
 
-@[simp] lemma models_rew {x : S} : S ⊧[x *> me] p.mlift ↔ S ⊧[me] p :=
+@[simp] lemma models_rew {x : S} : S ⊧[x .> me] p.mlift ↔ S ⊧[me] p :=
 by simp[val]
 
 end formula
 
-def sentence.val : sentence L → Prop := formula.val S fin.nil
+def models (S : Structure L) (p : formula L) : Prop := ∀ e, S ⊧[e] p
 
-def models (S : Structure L) (p : formula L m) : Prop := ∀ e, S ⊧[e] p
+instance : semantics (formula L) (Structure L) := ⟨models, by simp[models], by simp[models]⟩
 
-instance : semantics (formula L m) (Structure L) := ⟨models, by simp[models], by simp[models]⟩
+lemma models_def {S : Structure L} {p : formula L} : S ⊧ p ↔ (∀ e, S ⊧[e] p) := by refl
 
-lemma models_def {S : Structure L} {p : formula L m} : S ⊧ p ↔ (∀ e, S ⊧[e] p) := by refl
+abbreviation valid (p : subformula L 0) : Prop := semantics.valid (Structure L) p
 
-lemma sentence_models_def {S : Structure L} {p : sentence L} : S ⊧ p ↔ S ⊧[fin.nil] p := by simp[models_def, fin.nil]
+abbreviation satisfiable (p : subformula L 0) : Prop := semantics.satisfiable (Structure L) p
 
-abbreviation valid (p : subformula L m 0) : Prop := semantics.valid (Structure L) p
+lemma valid_def (p : formula L) : valid p ↔ ∀ S : Structure L, S ⊧ p := by refl
 
-abbreviation satisfiable (p : subformula L m 0) : Prop := semantics.satisfiable (Structure L) p
+lemma satisfiable_def (p : formula L) : satisfiable p ↔ ∃ S : Structure L, S ⊧ p := by refl
 
-lemma valid_def (p : formula L m) : valid p ↔ ∀ S : Structure L, S ⊧ p := by refl
+abbreviation Satisfiable (T : preTheory L) : Prop := semantics.Satisfiable (Structure L) T
 
-lemma satisfiable_def (p : formula L m) : satisfiable p ↔ ∃ S : Structure L, S ⊧ p := by refl
-
-abbreviation Satisfiable (T : preTheory L m) : Prop := semantics.Satisfiable (Structure L) T
-
-lemma Satisfiable_def (T : preTheory L m) : Satisfiable T ↔ ∃ S : Structure L, S ⊧ T := by refl
+lemma Satisfiable_def (T : preTheory L) : Satisfiable T ↔ ∃ S : Structure L, S ⊧ T := by refl
 
 namespace formula
-variables {S} {m}
+variables {S}
 
-@[simp] lemma models_mlift {p : formula L m} : S ⊧ p.mlift ↔ S ⊧ p :=
+@[simp] lemma models_mlift {p : formula L} : S ⊧ p.mlift ↔ S ⊧ p :=
 by{ simp[models_def], split,
     { intros h e,
-      have : S ⊧[default *> e] p.mlift, from h _,
+      have : S ⊧[default .> e] p.mlift, from h _,
       exact models_rew.mp this },
-    { intros h e, rw ←fin.left_concat_eq e, simpa using h (e ∘ fin.succ)} }
+    { intros h e, rw ←nat.left_concat_eq e, simpa using h (e ∘ nat.succ)} }
 
 end formula
 
-namespace sentence
-variables {S} {p q : sentence L}
-
-@[simp] lemma models_verum : S ⊧ (⊤ : sentence L) := by simp[sentence_models_def]
-
-@[simp] lemma models_relation {k} (r : L.pr k) (v : fin k → subterm L 0 0) :
-  S ⊧ (relation r v) ↔ S.pr r (subterm.val S fin.nil fin.nil ∘ v) := by simp[sentence_models_def]
-
-@[simp] lemma models_imply : S ⊧ p ⟶ q ↔ (S ⊧ p → S ⊧ q) := by simp[sentence_models_def]
-
-@[simp] lemma models_neg : S ⊧ ∼p ↔ ¬S ⊧ p := by simp[sentence_models_def]
-
-@[simp] lemma models_and : S ⊧ p ⊓ q ↔ S ⊧ p ∧ S ⊧ q := by simp[sentence_models_def]
-
-@[simp] lemma models_or : S ⊧ p ⊔ q ↔ S ⊧ p ∨ S ⊧ q := by simp[sentence_models_def]
-
-@[simp] lemma models_iff : S ⊧ p ⟷ q ↔ (S ⊧ p ↔ S ⊧ q) := by simp[sentence_models_def]
-
-@[simp] lemma not_valid_iff_satisfiable (p : sentence L) : ¬valid p ↔ satisfiable (∼p) :=
-by simp[valid_def, satisfiable_def]
-
-end sentence
-
 namespace preTheory
-variables {S} {m} {T : preTheory L m}
+variables {S} {T : preTheory L}
 
 @[simp] lemma models_mlift : S ⊧ T.mlift ↔ S ⊧ T :=
 ⟨by { intros h p hp,
@@ -265,35 +238,35 @@ variables {S} {m} {T : preTheory L m}
 
 end preTheory
 
-instance : has_double_turnstile (preTheory L m) (formula L m) := ⟨semantics.consequence (Structure L)⟩
+instance : has_double_turnstile (preTheory L) (formula L) := ⟨semantics.consequence (Structure L)⟩
 
-lemma consequence_def {T : preTheory L m} {p : formula L m} :
+lemma consequence_def {T : preTheory L} {p : formula L} :
   T ⊧ p ↔ (∀ S : Structure L, S ⊧ T → S ⊧ p) := by refl
 
 variables {S}
 
-theorem soundness {T : preTheory L m} {p} : T ⊢ p → T ⊧ p := λ h,
+theorem soundness {T : preTheory L} {p} : T ⊢ p → T ⊧ p := λ h,
 begin
   apply provable.rec_on h,
-  { intros m T p b IH S hT me,
+  { intros T p b IH S hT me,
     simp[formula.val], intros x,
     have : S ⊧ p, from @IH S (by simpa using hT),
-    exact this (x *> me) },
-  { intros m T p q b₁ b₂ m₁ m₂ S hT me,
+    exact this (x .> me) },
+  { intros T p q b₁ b₂ m₁ m₂ S hT me,
     have h₁ : S ⊧[me] p → S ⊧[me] q, by simpa using m₁ hT me,
     have h₂ : S ⊧[me] p, from m₂ hT me,
     exact h₁ h₂ },
-  { intros m T p hp S hS, exact hS hp },
-  { intros m T S h me, simp },
-  { intros m T p q S hS me, simp, intros h _, exact h },
-  { intros m T p q r S hS me, simp,  intros h₁ h₂ h₃, exact h₁ h₃ (h₂ h₃) },
-  { intros m T p q S hS me, simp, intros h₁, contrapose, exact h₁ },
-  { intros m T p t S hS me, simp, intros h, exact h _ },
-  { intros m T p q S hS me, simp, intros h₁ h₂ x, exact h₁ x h₂ },
-  { intros m T S hS me, simp }
+  { intros T p hp S hS, exact hS hp },
+  { intros T S h me, simp },
+  { intros T p q S hS me, simp, intros h _, exact h },
+  { intros T p q r S hS me, simp,  intros h₁ h₂ h₃, exact h₁ h₃ (h₂ h₃) },
+  { intros T p q S hS me, simp, intros h₁, contrapose, exact h₁ },
+  { intros T p t S hS me, simp, intros h, exact h _ },
+  { intros T p q S hS me, simp, intros h₁ h₂ x, exact h₁ x h₂ },
+  { intros T S hS me, simp }
 end
 
-instance : logic.sound (formula L m) (Structure L) :=
+instance : logic.sound (formula L) (Structure L) :=
 ⟨λ T p, soundness⟩
 
 namespace Structure
@@ -319,12 +292,12 @@ lemma map_fn {k} (f : L₁.fn k) (v : fin k → S₁) : F (S₁.fn f v) = S₂.f
 
 lemma map_pr {k} (r : L₁.pr k) (v : fin k → S₁) : S₁.pr r v ↔ S₂.pr (τ.pr _ r) (F ∘ v) := F.map_pr' r v
 
-lemma map_val (me : fin m → S₁) (e : fin n → S₁) (t : subterm L₁ m n) :
+lemma map_val (me : ℕ → S₁) (e : fin n → S₁) (t : subterm L₁ n) :
   F (subterm.val S₁ me e t) = subterm.val S₂ (F ∘ me) (F ∘ e) (subterm.of_lhom τ t) :=
 by { induction t; simp,
      case function : k f v IH { simp[map_fn], refine congr_arg _ (by funext i; exact IH i) } }
 
-lemma val_iff_of_surjective (surj : function.surjective F) (me : fin m → S₁) : ∀ {n} (e : fin n → S₁) (p : subformula L₁ m n),
+lemma val_iff_of_surjective (surj : function.surjective F) (me : ℕ → S₁) : ∀ {n} (e : fin n → S₁) (p : subformula L₁ n),
   subformula.val S₁ me e p ↔ subformula.val S₂ (F ∘ me) (F ∘ e) (of_lhom τ p)
 | n e verum          := by simp[top_eq]
 | n e (relation r v) := by simp[map_pr F]; refine (iff_of_eq $ congr_arg _ $ funext $ by simp[map_val])
@@ -351,11 +324,11 @@ lemma val_iff_of_surjective (surj : function.surjective F) (me : fin m → S₁)
         exact (val_iff_of_surjective (x *> e) p).mpr (by simpa[fin.comp_left_concat] using h (F x)) }
     end
 
-lemma formula_val_iff_of_surjective (surj : function.surjective F) (me : fin m → S₁) (p : formula L₁ m) :
+lemma formula_val_iff_of_surjective (surj : function.surjective F) (me : ℕ → S₁) (p : formula L₁) :
   S₁ ⊧[me] p ↔ S₂ ⊧[F ∘ me] of_lhom τ p :=
 by simpa[show F ∘ fin.nil = fin.nil, from funext (by simp)] using val_iff_of_surjective F surj me fin.nil p
 
-lemma models_iff_of_surjective (surj : function.surjective F) (p : formula L₁ m) :
+lemma models_iff_of_surjective (surj : function.surjective F) (p : formula L₁) :
   S₁ ⊧ p ↔ S₂ ⊧ of_lhom τ p :=
 begin
   simp[models_def], split,
@@ -368,7 +341,7 @@ begin
     exact (formula_val_iff_of_surjective F surj me p).mpr (h (F ∘ me)) }
 end
 
-lemma val_iff_of_open (me : fin m → S₁) : ∀ {n} (e : fin n → S₁) (p : subformula L₁ m n) (hp : p.is_open),
+lemma val_iff_of_open (me : ℕ → S₁) : ∀ {n} (e : fin n → S₁) (p : subformula L₁ n) (hp : p.is_open),
   subformula.val S₁ me e p ↔ subformula.val S₂ (F ∘ me) (F ∘ e) (subformula.of_lhom τ p)
 | n e verum          _  := by simp[top_eq]
 | n e (relation r v) _  := by simp[map_pr F]; refine (iff_of_eq $ congr_arg _ $ funext $ by simp[map_val])
@@ -387,17 +360,18 @@ lemma val_iff_of_open (me : fin m → S₁) : ∀ {n} (e : fin n → S₁) (p : 
   end
 | n e (fal p)        hp := by exfalso; simpa using hp
 
-lemma formula_val_iff_of_open (me : fin m → S₁) (p : formula L₁ m) (hp : p.is_open) :
+lemma formula_val_iff_of_open (me : ℕ → S₁) (p : formula L₁) (hp : p.is_open) :
   S₁ ⊧[me] p ↔ S₂ ⊧[F ∘ me] subformula.of_lhom τ p :=
 by simpa[show F ∘ fin.nil = fin.nil, from funext (by simp)] using F.val_iff_of_open me fin.nil p hp
 
-lemma models_iff (me : fin m → S₁) (p : subformula L₁ m n) (hp : p.is_open) :
+lemma models_iff (me : ℕ → S₁) (p : subformula L₁ n) (hp : p.is_open) :
   S₂ ⊧[F ∘ me] subformula.of_lhom τ (∀'*p) → S₁ ⊧[me] ∀'*p :=
 by simp[formula.val]; intros h e; exact (F.val_iff_of_open me e p hp).mpr (h (F ∘ e))
 
-lemma models_of_lhom (F : S₁ →ₛ[τ] S₂) (p : subformula L₁ 0 n) (hp : p.is_open) :
+lemma models_of_lhom (F : S₁ →ₛ[τ] S₂) (p : subformula L₁ n) (hp : p.is_open) :
   S₂ ⊧ subformula.of_lhom τ (∀'*p) → S₁ ⊧ ∀'*p :=
-by simpa only [sentence_models_def, show F ∘ fin.nil = fin.nil, from funext (by simp)] using F.models_iff fin.nil p hp
+by { simp only [models_def, show F ∘ fin.nil = fin.nil, from funext (by simp)], intros h e, 
+     exact F.models_iff e p hp (h _)  }
 
 end hom
 
@@ -413,15 +387,15 @@ def of_lfin : S₂.restrict τ →ₛ[τ] S₂ :=
   map_fn' := by intros; refl,
   map_pr' := by intros; refl }
 
-lemma of_lfin.val_iff (me) {n} (e) (p : subformula L₁ m n) :
+lemma of_lfin.val_iff (me) {n} (e) (p : subformula L₁ n) :
   subformula.val (S₂.restrict τ) me e p ↔ subformula.val S₂ (S₂.of_lfin τ ∘ me) (S₂.of_lfin τ ∘ e) (subformula.of_lhom τ p) :=
 (S₂.of_lfin τ).val_iff_of_surjective function.surjective_id me e p
 
-lemma of_lfin.formula_val_iff (me) (p : formula L₁ m) :
+lemma of_lfin.formula_val_iff (me) (p : formula L₁) :
   S₂.restrict τ ⊧[me] p ↔ S₂ ⊧[S₂.of_lfin τ ∘ me] subformula.of_lhom τ p :=
 (S₂.of_lfin τ).formula_val_iff_of_surjective function.surjective_id me p
 
-lemma of_lfin.models_iff (p : formula L₁ m) :
+lemma of_lfin.models_iff (p : formula L₁) :
   S₂.restrict τ ⊧ p ↔ S₂ ⊧ subformula.of_lhom τ p :=
 (S₂.of_lfin τ).models_iff_of_surjective function.surjective_id p
 
